src/coq/Error.v
@@ -34,3 +34,7 @@ Arguments trywith _ _ _ _ _: simpl nomatch.
 Definition failwith {A:Type} {F} `{Monad F} `{MonadExc string F} (s:string) : F A := raise s.
 Hint Unfold failwith.
 Arguments failwith _ _ _ _: simpl nomatch.
+
+Definition undef := err.
+Definition undef_or_err := eitherT string err.
+
